small update

trillium/program_logic/adequacy_cond.v
@@ -10,20 +10,6 @@ From trillium.program_logic Require Export adequacy_utils.
 Set Default Proof Using "Type".
 Import uPred.
 
-Definition config_wp `{!irisG Λ M Σ} : iProp Σ :=
-  □ ∀ ex atr c1 σ2 ,
-      ⌜valid_exec ex⌝ →
-      ⌜trace_ends_in ex c1⌝ →
-      ⌜config_step c1.2 σ2⌝ →
-      state_interp ex atr ={⊤,∅}=∗ |={∅}▷=>^(S $ trace_length ex) |={∅,⊤}=>
-         ∃ δ2 ℓ, state_interp (trace_extend ex None (c1.1, σ2))
-                              (trace_extend atr ℓ δ2).
-
-#[global] Instance config_wp_persistent `{!irisG Λ M Σ} : Persistent config_wp.
-Proof. apply _. Qed.
-
-#[global] Typeclasses Opaque config_wp.
-
 
 (* the guarded definition of simulation. *)
 Definition Gsim_cond_pre Σ {Λ} (M : Model) (s : stuckness)
@@ -54,7 +40,7 @@ Definition Gsim_cond Σ {Λ} (M : Model) (s : stuckness)
   execution_trace Λ → auxiliary_trace M → iProp Σ :=
   fixpoint (Gsim_cond_pre Σ M s ξ C).
 
-#[global] Instance is_except_0_wptp {Σ} Λ M s ξ C ex sm:
+#[global] Instance is_except_0_Gsim_cond {Σ} Λ M s ξ C ex sm:
   IsExcept0 (@Gsim_cond Σ Λ M s ξ C ex sm).
 Proof.
   rewrite /IsExcept0; iIntros "H".
@@ -90,98 +76,6 @@ Proof.
   iDestruct "H" as (δ' ℓ) "H".
   iExists _, _. iApply "IH"; done.
 Qed.
-
-Section adequacy_helper_lemmas.
-  Context `{!irisG Λ M Σ}.
-
-  Lemma take_step s Φs ex atr c c' oζ:
-    valid_exec ex →
-    trace_ends_in ex c →
-    locale_step c oζ c' →
-    config_wp -∗
-    state_interp ex atr -∗
-    wptp s c.1 Φs ={⊤,∅}=∗ |={∅}▷=>^(S (trace_length ex))
-                                             |={∅,⊤}=>
-    ⌜∀ e2, s = NotStuck → e2 ∈ c'.1 → not_stuck e2 c'.2⌝ ∗
-    ∃ δ' ℓ,
-      state_interp (trace_extend ex oζ c') (trace_extend atr ℓ δ') ∗
-      wptp s  c'.1 (Φs ++ newposts c.1 c'.1). 
-  Proof.
-    iIntros (Hexvalid Hexe Hstep) "config_wp HSI Hc1".
-    inversion Hstep as
-        [ρ1 ρ2 e1 σ1 e2 σ2 efs t1 t2 -> -> Hpstep | ρ1 ρ2 σ1 σ2 t -> -> Hcfgstep].
-    - rewrite /= !prefixes_from_app.
-      iDestruct (big_sepL2_app_inv_l with "Hc1") as
-          (Φs1 Φs2') "[-> [Ht1 Het2]]".
-      iDestruct (big_sepL2_cons_inv_l with "Het2") as (Φ Φs2) "[-> [He Ht2]]".
-      iDestruct (wp_take_step with "HSI He") as "He"; [done|done|done|done|].
-      iMod "He" as "He". iModIntro. iMod "He" as "He". iModIntro. iNext.
-      iMod "He" as "He". iModIntro.
-      iApply (step_fupdN_wand with "[He]"); first by iApply "He".
-      iIntros "He".
-      iMod "He" as (δ' ℓ) "(HSI & He2 & Hefs) /=".
-      have Heq: forall a b c d, a ++ e1 :: c ++ d = (a ++ e1 :: c) ++ d.
-      { intros **. by list_simplifier. }
-      iAssert (wptp_from (t1 ++ e2 :: t2) s efs (newposts (t1 ++ e2 :: t2) ((t1 ++ e2 :: t2) ++ efs)))
-        with "[Hefs]" as "Hefs".
-      { rewrite -new_threads_wptp_from. iApply (big_sepL_impl with "Hefs").
-        iIntros "!#" (i e Hin) "Hwp". list_simplifier.
-        erewrite locale_equiv; first by iFrame.
-        apply locales_equiv_middle. erewrite locale_step_preserve =>//. }
-      assert (valid_exec (ex :tr[Some (locale_of t1 e1)]: (t1 ++ e2 :: t2 ++ efs, σ2))).
-      { econstructor; eauto. }
-      iMod (wptp_not_stuck_same _ _ σ2 _ _ [] with "HSI Hefs") as "[HSI [Hefs %]]"; [done| | ].
-      { list_simplifier. done. }
-      iMod (wptp_not_stuck_same _ _ σ2 _ _ (e2 :: (t2 ++ efs)) with "HSI Ht1") as "[HSI [Ht1 %]]"; [done|  |].
-      {  list_simplifier. done. }
-      iMod (wptp_not_stuck _ _ σ2 _ (t1 ++ [e2]) _ efs with "HSI Ht2") as "[HSI [Ht2 %]]"; [| done | |].
-      { rewrite !prefixes_from_app. apply Forall2_app.
-        - apply locales_equiv_refl.
-        - constructor; last constructor. list_simplifier. erewrite <-locale_step_preserve =>//. }
-      { list_simplifier. done. }
-      iMod (wp_not_stuck _ _ ectx_emp with "HSI He2") as "[HSI [He2 %]]";
-        [done|by rewrite ectx_fill_emp|by erewrite <-locale_step_preserve|].
-
-      iDestruct (wptp_app with "Ht2 Hefs") as "Ht2efs".
-      { by list_simplifier. }
-      erewrite (locale_step_preserve e1 e2) =>//.
-      iDestruct (wptp_cons_l with "He2 Ht2efs") as "He2t2efs".
-      iDestruct (wptp_app with "Ht1 He2t2efs") as "Hc2"; [by list_simplifier|].
-      iDestruct (wptp_of_val_post with "Hc2") as "Hc2".
-      iMod (pre_step_elim with "HSI Hc2") as "[HSI [Hc2posts Hc2back]]".
-      iModIntro; simpl in *.
-      iSplit.
-      { iPureIntro; set_solver. }
-      iExists δ', ℓ.
-      rewrite -!app_assoc.
-      iFrame.
-      list_simplifier.
-      erewrite newposts_locales_equiv;
-        [iFrame | apply locales_equiv_middle; erewrite <-locale_step_preserve =>//].
-      iDestruct ("Hc2back" with "[$]") as "X". iFrame. 
-      rewrite prefixes_from_app //.
-    - rewrite /= /config_wp.
-      iDestruct ("config_wp" with "[] [] [] HSI") as "Hcfg"; [done|done|done|].
-      iMod "Hcfg". iModIntro. iMod "Hcfg". iModIntro.
-      iNext. iMod "Hcfg". iModIntro.
-      iApply (step_fupdN_wand with "[Hcfg]"); first by iApply "Hcfg".
-      iIntros "Hcfg".
-      iMod "Hcfg" as (δ2 ℓ) "HSI".
-      assert (valid_exec (ex :tr[None]: ((t, σ1).1, σ2))).
-      { econstructor; eauto. }
-      iMod (wptp_not_stuck _ _ σ2 _ _ _ [] with "HSI Hc1") as "[HSI [Hc1 %]]";
-        [apply locales_equiv_refl|done|by list_simplifier|].
-      iDestruct (wptp_of_val_post with "Hc1") as "Hc1".
-      iMod (pre_step_elim with "HSI Hc1") as "[HSI [Hc1posts Hc1back]]".
-      iModIntro.
-      iSplit; first by auto.
-      iExists δ2, ℓ.
-      rewrite newposts_same_empty. list_simplifier.
-      iFrame.
-      by iApply "Hc1back". 
-  Qed.
-
-End adequacy_helper_lemmas.
 
 
 Definition all_posts `{irisG Λ M Σ} (tp: list (expr Λ)) es
@@ -288,16 +182,11 @@ Section StrongAdequacyHelpers.
   Context (post : locale Λ → val Λ → iProp Σ).
 
   Context (C: execution_trace Λ → Prop).
-  Hypothesis C_DEC: forall ex, Decision (C ex). 
+  Hypothesis C_DEC: forall ex, Decision (C ex).
 
   Definition cur_tr_repr_impl
     (Hinv : invGS_gen HasNoLc Σ)    
-(i :=
-    {|
-      iris_invGS := Hinv;
-      state_interp := stateI;
-      fork_post := post
-    |} : irisG Λ M Σ)
+(i := {| iris_invGS := Hinv; state_interp := stateI; fork_post := post |} : irisG Λ M Σ)
     s es Φs ex atr: iProp Σ :=
     (
     let c1 := trace_last ex in 
@@ -308,12 +197,7 @@ Section StrongAdequacyHelpers.
 
   Definition cur_tr_repr
     (Hinv : invGS_gen HasNoLc Σ)    
-(i :=
-    {|
-      iris_invGS := Hinv;
-      state_interp := stateI;
-      fork_post := post
-    |} : irisG Λ M Σ)
+(i := {| iris_invGS := Hinv; state_interp := stateI; fork_post := post |} : irisG Λ M Σ)
     s es Φs ex atr: iProp Σ :=
     ⌜ C ex ⌝ → cur_tr_repr_impl _ s es Φs ex atr.
 
@@ -353,12 +237,7 @@ Section StrongAdequacyHelpers.
   (* TODO: better name *)
   Local Lemma locales_rewrite
     (Hinv : invGS_gen HasNoLc Σ)
-    (i :=
-    {|
-      iris_invGS := Hinv;
-      state_interp := stateI;
-      fork_post := post
-    |} : irisG Λ M Σ)
+    (i := {| iris_invGS := Hinv; state_interp := stateI; fork_post := post |} : irisG Λ M Σ)
     (* (R: list (expr Λ) → expr Λ -> iProp Σ) *)
     es
     (tp : list (expr Λ))
